Pev1.v
@@ -1,0 +1,51 @@
+From Stdlib Require Import ZArith Ascii List String PrimInt63.
+From Stdlib Require Import -(notations) PArray.
+From mathcomp Require Import all_boot.
+From HB Require Import structures.
+
+From Stdlib Require Import Lia.
+Require Import ssr_int.
+Require Import Pbasic.
+Require Import Pmoves.
+Require Import Phash.
+Require Import Palphabeta.
+Require Import FourInARow.
+
+(******************************************************************************)
+(*                                                                            *)
+(*                                                                            *)
+(*    First position                                                          *)
+(*                                                                            *)
+(*                                                                            *)
+(******************************************************************************)
+
+
+Import PrimInt63Notations.
+Import Uint63Axioms.
+Import Uint63.
+Open Scope uint63_scope.
+
+Definition ev1 := (
+                 "_______"
+              ++ "_______"
+              ++ "_______"
+              ++ "_______"
+              ++ "_______"
+              ++ "O__X___")%string.
+
+Definition ew1 :=  (get_position ev1).1.
+Definition eb1 :=  (get_position ev1).2.
+
+Lemma eval_ev1E : top_eval ew1 eb1 = win.
+Proof.
+(* vm_cast_no_check (refl_equal win). *)
+Admitted.
+
+Lemma eval_ev1 : eval ew1 eb1 = WIN.
+Proof.
+suff : valid_eval ew1 eb1 win.
+  by rewrite /valid_eval; case/or3P: (evalOr ew1 eb1) => /eqP->.
+rewrite -eval_ev1E.
+by apply: topeval_correct.
+Qed.
+
